theories/zoo_persistent/sstore_1.v
@@ -11,9 +11,9 @@ From zoo_std Require Import
   list.
 From zoo_persistent Require Export
   base
-  pstore_1__code.
+  sstore_1__code.
 From zoo_persistent Require Import
-  pstore_1__types.
+  sstore_1__types.
 From zoo Require Import
   options.
 
@@ -553,22 +553,22 @@ End adiffl.
 (* ------------------------------------------------------------------------ *)
 (* Proof. *)
 
-Class Pstore1G Σ `{zoo_G : !ZooG Σ} :=
-  { #[local] pstore_1_G_set_G :: MonoGsetG Σ (location * gmap location val)%type
+Class Sstore1G Σ `{zoo_G : !ZooG Σ} :=
+  { #[local] sstore_1_G_set_G :: MonoGsetG Σ (location * gmap location val)%type
   }.
 
-Definition pstore_1_Σ :=
+Definition sstore_1_Σ :=
   #[mono_gset_Σ (location * gmap location val)%type
   ].
-#[global] Instance subG_pstore_1_Σ Σ `{zoo_G : !ZooG Σ} :
-  subG pstore_1_Σ Σ →
-  Pstore1G Σ.
+#[global] Instance subG_sstore_1_Σ Σ `{zoo_G : !ZooG Σ} :
+  subG sstore_1_Σ Σ →
+  Sstore1G Σ.
 Proof.
   solve_inG.
 Qed.
 
-Section pstore_1_G.
-  Context `{pstore_1_G : Pstore1G Σ}.
+Section sstore_1_G.
+  Context `{sstore_1_G : Sstore1G Σ}.
 
   Notation diff := (
     (* location and its old value. *)
@@ -604,9 +604,9 @@ Section pstore_1_G.
   Definition snapshot_inv (M:map_model) (C:gset (location * gmap location val)) :=
     ∀ l σ, (l,σ) ∈ C → ∃ σ', M !! l = Some σ' ∧ σ ⊆ σ'.
 
-  #[local] Definition pstore_1_map_auth (γ:gname) (s:gset (location*(gmap location val))) :=
+  #[local] Definition sstore_1_map_auth (γ:gname) (s:gset (location*(gmap location val))) :=
     mono_gset_auth γ (DfracOwn 1) s.
-  #[local] Definition pstore_1_map_elem γ l σ :=
+  #[local] Definition sstore_1_map_elem γ l σ :=
     mono_gset_elem γ (l,σ).
 
   Lemma extract_unaliased (g : graph_store) :
@@ -628,9 +628,9 @@ Section pstore_1_G.
 
   #[local] Definition snapshosts_model (t0:location) (M:map_model) : iProp Σ :=
     ∃ (γ:gname) (C:gset (location * gmap location val)), (* the model of snapshots *)
-      ⌜snapshot_inv M C⌝ ∗ t0 ↪ γ ∗ pstore_1_map_auth γ C.
+      ⌜snapshot_inv M C⌝ ∗ t0 ↪ γ ∗ sstore_1_map_auth γ C.
 
-  #[local] Definition pstore_1 (t:val) (σ:gmap location val) : iProp Σ :=
+  #[local] Definition sstore_1 (t:val) (σ:gmap location val) : iProp Σ :=
     ∃ (t0 r:location)
       (σ0:gmap location val) (* the global map, with all the points-to ever allocated *)
       (g:graph_store) (* the global graph *)
@@ -645,30 +645,30 @@ Section pstore_1_G.
   Definition open_inv : string :=
     "[%t0 [%r [%σ0 [%g [%M ((->&%Hinv&%Hcoh&%Hgraph)&Ht0&Hr&HC&Hσ0&Hg)]]]]]".
 
-  Definition pstore_1_snapshot t s σ : iProp Σ :=
-    ∃ γ (t0:location) l, ⌜t=#t0 ∧ s=ValTuple [t;#l]⌝ ∗ t0 ↪ γ ∗ pstore_1_map_elem γ l σ.
+  Definition sstore_1_snapshot t s σ : iProp Σ :=
+    ∃ γ (t0:location) l, ⌜t=#t0 ∧ s=ValTuple [t;#l]⌝ ∗ t0 ↪ γ ∗ sstore_1_map_elem γ l σ.
 
-  #[global] Instance pstore_1_snapshot_timeless t s σ :
-    Timeless (pstore_1_snapshot t s σ).
+  #[global] Instance sstore_1_snapshot_timeless t s σ :
+    Timeless (sstore_1_snapshot t s σ).
   Proof.
     apply _.
   Qed.
 
-  #[global] Instance pstore_1_snapshot_persistent t s σ :
-    Persistent (pstore_1_snapshot t s σ).
+  #[global] Instance sstore_1_snapshot_persistent t s σ :
+    Persistent (sstore_1_snapshot t s σ).
   Proof.
     apply _.
   Qed.
 
-  Lemma pstore_1٠create𑁒spec :
+  Lemma sstore_1٠create𑁒spec :
     {{{
       True
     }}}
-      pstore_1٠create ()
+      sstore_1٠create ()
     {{{
       t
     , RET t;
-        pstore_1 t ∅
+        sstore_1 t ∅
     }}}.
   Proof.
     iIntros "%Φ _ HΦ".
@@ -704,16 +704,16 @@ Section pstore_1_G.
     apply He in H. set_solver.
   Qed.
 
-  Lemma pstore_1٠ref𑁒spec t σ v :
+  Lemma sstore_1٠ref𑁒spec t σ v :
     {{{
-      pstore_1 t σ
+      sstore_1 t σ
     }}}
-      pstore_1٠ref t v
+      sstore_1٠ref t v
     {{{
       l
     , RET #l;
       ⌜l ∉ dom σ⌝ ∗
-      pstore_1 t (<[l := v]> σ)
+      sstore_1 t (<[l := v]> σ)
     }}}.
   Proof.
     iIntros (ϕ) open_inv. iIntros "HΦ".
@@ -769,15 +769,15 @@ Section pstore_1_G.
       apply not_elem_of_dom in Hl0. set_solver. }
   Qed.
 
-  Lemma pstore_1٠get𑁒spec {t σ l} v :
+  Lemma sstore_1٠get𑁒spec {t σ l} v :
     σ !! l = Some v →
     {{{
-      pstore_1 t σ
+      sstore_1 t σ
     }}}
-      pstore_1٠get t #l
+      sstore_1٠get t #l
     {{{
       RET v;
-      pstore_1 t σ
+      sstore_1 t σ
     }}}.
   Proof.
     iIntros (Hl ϕ) open_inv. iIntros "HΦ".
@@ -790,15 +790,15 @@ Section pstore_1_G.
     iStepFrameSteps 8.
   Qed.
 
-  Lemma pstore_1٠set𑁒spec t σ l v :
+  Lemma sstore_1٠set𑁒spec t σ l v :
     l ∈ dom σ →
     {{{
-      pstore_1 t σ
+      sstore_1 t σ
     }}}
-      pstore_1٠set t #l v
+      sstore_1٠set t #l v
     {{{
       RET ();
-      pstore_1 t (<[l := v]> σ)
+      sstore_1 t (<[l := v]> σ)
     }}}.
   Proof.
     iIntros (Hl Φ) open_inv. iIntros "HΦ".
@@ -874,16 +874,16 @@ Section pstore_1_G.
       rewrite lookup_insert_ne //. eauto. }
   Qed.
 
-  Lemma pstore_1٠capture𑁒spec t σ :
+  Lemma sstore_1٠capture𑁒spec t σ :
     {{{
-      pstore_1 t σ
+      sstore_1 t σ
     }}}
-      pstore_1٠capture t
+      sstore_1٠capture t
     {{{
       s
     , RET s;
-      pstore_1 t σ ∗
-      pstore_1_snapshot t s σ
+      sstore_1 t σ ∗
+      sstore_1_snapshot t s σ
     }}}.
   Proof.
     iIntros (Φ) open_inv. iIntros "HΦ".
@@ -903,14 +903,14 @@ Section pstore_1_G.
   Definition fsts  (ys:list (location*(location*val)*location)) : list val :=
     (fun '(x,_,_) => ValLoc x) <$> ys.
 
-  Lemma pstore_1٠collect𑁒spec_aux (r r':location) t' (xs:list val) (ys:list (location*(location*val)*location)) (g:graph_store) :
+  Lemma sstore_1٠collect𑁒spec_aux (r r':location) t' (xs:list val) (ys:list (location*(location*val)*location)) (g:graph_store) :
     list_model' t' xs →
     path g r ys r' →
     {{{
       r' ↦ᵣ §Root ∗
       ([∗ set] '(r, (l, v), r') ∈ g, r ↦ᵣ ‘Diff( #(l : location), v, #(r' : location) ))
     }}}
-      pstore_1٠collect #r t'
+      sstore_1٠collect #r t'
     {{{
       t
     , RET (#r',t);
@@ -932,13 +932,13 @@ Section pstore_1_G.
     }
   Qed.
 
-  Lemma pstore_1٠collect𑁒spec (r r':location) (ys:list (location*(location*val)*location)) (g:graph_store) :
+  Lemma sstore_1٠collect𑁒spec (r r':location) (ys:list (location*(location*val)*location)) (g:graph_store) :
     path g r ys r' →
     {{{
       r' ↦ᵣ §Root ∗
       ([∗ set] '(r, (l, v), r') ∈ g, r ↦ᵣ ‘Diff( #(l : location), v, #(r' : location) ))
     }}}
-      pstore_1٠collect #r []
+      sstore_1٠collect #r []
     {{{
       t
     , RET (#r',t);
@@ -948,7 +948,7 @@ Section pstore_1_G.
     }}}.
   Proof.
     iIntros (? Φ) "(?&?) HΦ".
-    iDestruct (pstore_1٠collect𑁒spec_aux with "[$]") as "Go"; [done.. |].
+    iDestruct (sstore_1٠collect𑁒spec_aux with "[$]") as "Go"; [done.. |].
     rewrite -list_to_val_nil.
     iApply "Go". rewrite -rev_alt //.
   Qed.
@@ -1001,7 +1001,7 @@ Section pstore_1_G.
     induction 1; eauto using mirror_cons,mirror_nil.
   Qed.
 
-  Lemma pstore_1٠revert𑁒spec_aux g g1 r t g2 xs r' w σ σ0 :
+  Lemma sstore_1٠revert𑁒spec_aux g g1 r t g2 xs r' w σ σ0 :
     list_model' t (fsts (rev xs)) →
     locations_of_edges_in g2 (dom σ) →
     g2 = list_to_set xs →
@@ -1014,7 +1014,7 @@ Section pstore_1_G.
       ([∗ set] '(r, (l, v), r') ∈ g1, r ↦ᵣ ‘Diff( #(l : location), v, #(r' : location) )) ∗
       ([∗ set] '(r, (l, v), r') ∈ g2, r ↦ᵣ ‘Diff( #(l : location), v, #(r' : location) ))
     }}}
-      pstore_1٠revert #r' t
+      sstore_1٠revert #r' t
     {{{
       RET ();
       ∃ ys,
@@ -1076,7 +1076,7 @@ Section pstore_1_G.
     }
   Qed.
 
-  Lemma pstore_1٠revert𑁒spec r t g xs r' w σ σ0 :
+  Lemma sstore_1٠revert𑁒spec r t g xs r' w σ σ0 :
     list_model' t (fsts (rev xs)) →
     locations_of_edges_in g (dom σ) →
     g = list_to_set xs →
@@ -1087,7 +1087,7 @@ Section pstore_1_G.
       ([∗ map] l0↦v0 ∈ σ, l0 ↦ᵣ v0) ∗
       ([∗ set] '(r, (l, v), r') ∈ g, r ↦ᵣ ‘Diff( #(l : location), v, #(r' : location) ))
     }}}
-      pstore_1٠revert #r' t
+      sstore_1٠revert #r' t
     {{{
       RET ();
       ∃ ys,
@@ -1098,7 +1098,7 @@ Section pstore_1_G.
     }}}.
   Proof.
     iIntros (->???? Φ) "(?&?&?) HΦ".
-    iApply (pstore_1٠revert𑁒spec_aux g ∅ with "[-HΦ]"); try done.
+    iApply (sstore_1٠revert𑁒spec_aux g ∅ with "[-HΦ]"); try done.
     { rewrite big_sepS_empty. iFrame. }
     { iModIntro. iIntros "[% ?]". iApply "HΦ". iExists _. rewrite left_id_L //. }
   Qed.
@@ -1110,7 +1110,7 @@ Section pstore_1_G.
     rewrite IHxs /fsts fmap_app //.
   Qed.
 
-  Lemma pstore_1٠reroot𑁒spec r (xs:list (location*(location*val)*location)) r' g σ :
+  Lemma sstore_1٠reroot𑁒spec r (xs:list (location*(location*val)*location)) r' g σ :
     locations_of_edges_in g (dom σ) →
     g = list_to_set xs →
     acyclic g →
@@ -1120,7 +1120,7 @@ Section pstore_1_G.
       ([∗ map] l0↦v0 ∈ σ, l0 ↦ᵣ v0) ∗
       ([∗ set] '(r, (l, v), r') ∈ g, r ↦ᵣ ‘Diff( #(l : location), v, #(r' : location) ))
     }}}
-      pstore_1٠reroot #r
+      sstore_1٠reroot #r
     {{{
       RET ();
       ∃ ys,
@@ -1131,9 +1131,9 @@ Section pstore_1_G.
     }}}.
   Proof.
     iIntros (???? Φ) "(Hr'&Hσ&Hg) HΦ".
-    wp_rec. wp_apply (pstore_1٠collect𑁒spec with "[$]"). done.
+    wp_rec. wp_apply (sstore_1٠collect𑁒spec with "[$]"). done.
     iIntros (?) "(?&?&%Heq)". rewrite {}Heq.
-    wp_apply+ (pstore_1٠revert𑁒spec with "[-HΦ]"); try done; first rewrite rev_fsts //.
+    wp_apply+ (sstore_1٠revert𑁒spec with "[-HΦ]"); try done; first rewrite rev_fsts //.
     iSteps.
   Qed.
 
@@ -1529,7 +1529,7 @@ Section pstore_1_G.
   Lemma use_snapshots_model γ (t0:location) M r σ :
     t0 ↪ γ -∗
     snapshosts_model t0 M -∗
-    pstore_1_map_elem γ r σ -∗
+    sstore_1_map_elem γ r σ -∗
     ⌜exists σ1, M !! r = Some σ1 ∧ σ ⊆ σ1⌝.
   Proof.
     iIntros "Hmeta [%γ' [%C (%Hsnapshot&Hmeta'&HC)]] ?".
@@ -1539,15 +1539,15 @@ Section pstore_1_G.
     eauto.
   Qed.
 
-  Lemma pstore_1٠restore𑁒spec t σ s σ' :
+  Lemma sstore_1٠restore𑁒spec t σ s σ' :
     {{{
-      pstore_1 t σ ∗
-      pstore_1_snapshot t s σ'
+      sstore_1 t σ ∗
+      sstore_1_snapshot t s σ'
     }}}
-      pstore_1٠restore t s
+      sstore_1٠restore t s
     {{{
       RET ();
-      pstore_1 t σ'
+      sstore_1 t σ'
     }}}.
   Proof.
     iIntros (Φ) "(HI&Hsnapshot) HΦ".
@@ -1585,7 +1585,7 @@ Section pstore_1_G.
     rewrite (union_difference_L (list_to_set xs) g) //.
 
     iDestruct (big_sepS_union with "Hg") as "(Hxs&Hg)". set_solver.
-    wp_apply (pstore_1٠reroot𑁒spec with "[Hr Hxs Hσ0]").
+    wp_apply (sstore_1٠reroot𑁒spec with "[Hr Hxs Hσ0]").
     4:{ eapply path_restrict. done. }
     2:done.
     { destruct Hcoh as [_ X]. eapply locations_of_edges_weak; eauto. }
@@ -1648,10 +1648,10 @@ Section pstore_1_G.
       }
     }
   Qed.
-End pstore_1_G.
+End sstore_1_G.
 
 From zoo_persistent Require
-  pstore_1__opaque.
+  sstore_1__opaque.
 
-#[global] Opaque pstore_1.
-#[global] Opaque pstore_1_snapshot.
+#[global] Opaque sstore_1.
+#[global] Opaque sstore_1_snapshot.
