theories/zoo_persistent/parray_1__opaque.v
@@ -1,6 +1,0 @@
-From zoo_persistent Require Import
-  parray_1__code.
-
-#[global] Opaque parray_1٠make.
-#[global] Opaque parray_1٠get.
-#[global] Opaque parray_1٠set.
