theories/zoo_persistent/parray_2__opaque.v
@@ -1,8 +1,0 @@
-From zoo_persistent Require Import
-  parray_2__code.
-
-#[global] Opaque parray_2٠make.
-#[global] Opaque parray_2٠get.
-#[global] Opaque parray_2٠set.
-#[global] Opaque parray_2٠capture.
-#[global] Opaque parray_2٠restore.
