theories/zoo_persistent/parray__opaque.v
@@ -1,0 +1,6 @@
+From zoo_persistent Require Import
+  parray__code.
+
+#[global] Opaque parray٠make.
+#[global] Opaque parray٠get.
+#[global] Opaque parray٠set.
