theories/zoo_persistent/parray__types.v
@@ -9,19 +9,19 @@ From zoo Require Import
   options.
 
 Notation "'Root'" := (
-  in_type "zoo_persistent.parray_1.descr" 0
+  in_type "zoo_persistent.parray.descr" 0
 )(in custom zoo_tag
 ).
 Notation "'Diff'" := (
-  in_type "zoo_persistent.parray_1.descr" 1
+  in_type "zoo_persistent.parray.descr" 1
 )(in custom zoo_tag
 ).
 
 Notation "'equal'" := (
-  in_type "zoo_persistent.parray_1.descr.Root" 0
+  in_type "zoo_persistent.parray.descr.Root" 0
 )(in custom zoo_proj
 ).
 Notation "'data'" := (
-  in_type "zoo_persistent.parray_1.descr.Root" 1
+  in_type "zoo_persistent.parray.descr.Root" 1
 )(in custom zoo_proj
 ).
