theories/zoo_persistent/pstore_1__opaque.v
@@ -1,9 +1,0 @@
-From zoo_persistent Require Import
-  pstore_1__code.
-
-#[global] Opaque pstore_1٠create.
-#[global] Opaque pstore_1٠ref.
-#[global] Opaque pstore_1٠get.
-#[global] Opaque pstore_1٠set.
-#[global] Opaque pstore_1٠capture.
-#[global] Opaque pstore_1٠restore.
