theories/zoo_persistent/pstore_2__opaque.v
@@ -1,9 +1,0 @@
-From zoo_persistent Require Import
-  pstore_2__code.
-
-#[global] Opaque pstore_2٠create.
-#[global] Opaque pstore_2٠ref.
-#[global] Opaque pstore_2٠get.
-#[global] Opaque pstore_2٠set.
-#[global] Opaque pstore_2٠capture.
-#[global] Opaque pstore_2٠restore.
