theories/zoo_persistent/pstore__opaque.v
@@ -1,9 +1,0 @@
-From zoo_persistent Require Import
-  pstore__code.
-
-#[global] Opaque pstore٠create.
-#[global] Opaque pstore٠ref.
-#[global] Opaque pstore٠get.
-#[global] Opaque pstore٠set.
-#[global] Opaque pstore٠capture.
-#[global] Opaque pstore٠restore.
