theories/zoo_persistent/sarray__opaque.v
@@ -1,0 +1,8 @@
+From zoo_persistent Require Import
+  sarray__code.
+
+#[global] Opaque sarray٠make.
+#[global] Opaque sarray٠get.
+#[global] Opaque sarray٠set.
+#[global] Opaque sarray٠capture.
+#[global] Opaque sarray٠restore.
