theories/zoo_persistent/sarray__types.v
@@ -9,23 +9,23 @@ From zoo Require Import
   options.
 
 Notation "'Root'" := (
-  in_type "zoo_persistent.parray_2.descr" 0
+  in_type "zoo_persistent.sarray.descr" 0
 )(in custom zoo_tag
 ).
 Notation "'Diff'" := (
-  in_type "zoo_persistent.parray_2.descr" 1
+  in_type "zoo_persistent.sarray.descr" 1
 )(in custom zoo_tag
 ).
 
 Notation "'equal'" := (
-  in_type "zoo_persistent.parray_2.t" 0
+  in_type "zoo_persistent.sarray.t" 0
 )(in custom zoo_field
 ).
 Notation "'data'" := (
-  in_type "zoo_persistent.parray_2.t" 1
+  in_type "zoo_persistent.sarray.t" 1
 )(in custom zoo_field
 ).
 Notation "'root'" := (
-  in_type "zoo_persistent.parray_2.t" 2
+  in_type "zoo_persistent.sarray.t" 2
 )(in custom zoo_field
 ).
