theories/zoo_persistent/sstore_1__types.v
@@ -9,19 +9,19 @@ From zoo Require Import
   options.
 
 Notation "'Root'" := (
-  in_type "zoo_persistent.pstore_1.descr" 0
+  in_type "zoo_persistent.sstore_1.descr" 0
 )(in custom zoo_tag
 ).
 Notation "'Diff'" := (
-  in_type "zoo_persistent.pstore_1.descr" 1
+  in_type "zoo_persistent.sstore_1.descr" 1
 )(in custom zoo_tag
 ).
 
 Notation "'snapshot_store'" := (
-  in_type "zoo_persistent.pstore_1.snapshot" 0
+  in_type "zoo_persistent.sstore_1.snapshot" 0
 )(in custom zoo_proj
 ).
 Notation "'snapshot_root'" := (
-  in_type "zoo_persistent.pstore_1.snapshot" 1
+  in_type "zoo_persistent.sstore_1.snapshot" 1
 )(in custom zoo_proj
 ).
