theories/zoo_persistent/sstore_2__types.v
@@ -9,41 +9,41 @@ From zoo Require Import
   options.
 
 Notation "'ref_gen'" := (
-  in_type "zoo_persistent.pstore_2.ref" 0
+  in_type "zoo_persistent.sstore_2.ref" 0
 )(in custom zoo_field
 ).
 Notation "'ref_value'" := (
-  in_type "zoo_persistent.pstore_2.ref" 1
+  in_type "zoo_persistent.sstore_2.ref" 1
 )(in custom zoo_field
 ).
 
 Notation "'Root'" := (
-  in_type "zoo_persistent.pstore_2.descr" 0
+  in_type "zoo_persistent.sstore_2.descr" 0
 )(in custom zoo_tag
 ).
 Notation "'Diff'" := (
-  in_type "zoo_persistent.pstore_2.descr" 1
+  in_type "zoo_persistent.sstore_2.descr" 1
 )(in custom zoo_tag
 ).
 
 Notation "'gen'" := (
-  in_type "zoo_persistent.pstore_2.t" 0
+  in_type "zoo_persistent.sstore_2.t" 0
 )(in custom zoo_field
 ).
 Notation "'root'" := (
-  in_type "zoo_persistent.pstore_2.t" 1
+  in_type "zoo_persistent.sstore_2.t" 1
 )(in custom zoo_field
 ).
 
 Notation "'snapshot_store'" := (
-  in_type "zoo_persistent.pstore_2.snapshot" 0
+  in_type "zoo_persistent.sstore_2.snapshot" 0
 )(in custom zoo_proj
 ).
 Notation "'snapshot_gen'" := (
-  in_type "zoo_persistent.pstore_2.snapshot" 1
+  in_type "zoo_persistent.sstore_2.snapshot" 1
 )(in custom zoo_proj
 ).
 Notation "'snapshot_root'" := (
-  in_type "zoo_persistent.pstore_2.snapshot" 2
+  in_type "zoo_persistent.sstore_2.snapshot" 2
 )(in custom zoo_proj
 ).
