theories/zoo_persistent/suf__opaque.v
@@ -1,0 +1,10 @@
+From zoo_persistent Require Import
+  suf__code.
+
+#[global] Opaque suf٠create.
+#[global] Opaque suf٠make.
+#[global] Opaque suf٠repr.
+#[global] Opaque suf٠equiv.
+#[global] Opaque suf٠union.
+#[global] Opaque suf٠capture.
+#[global] Opaque suf٠restore.
