theories/zoo_persistent/suf__types.v
@@ -4,15 +4,15 @@ From zoo.language Require Import
   typeclasses
   notations.
 From zoo_persistent Require Import
-  pstore_2.
+  sstore_2.
 From zoo Require Import
   options.
 
 Notation "'Root'" := (
-  in_type "zoo_persistent.puf.descr" 0
+  in_type "zoo_persistent.suf.descr" 0
 )(in custom zoo_tag
 ).
 Notation "'Link'" := (
-  in_type "zoo_persistent.puf.descr" 1
+  in_type "zoo_persistent.suf.descr" 1
 )(in custom zoo_tag
 ).
